src/cddl/test/dpe/CDDLTest.DPEMain.fst
@@ -1,0 +1,120 @@
+module CDDLTest.DPEMain
+open Pulse.Lib
+open Pulse.Lib.Pervasives
+// open DPETypes
+// open EngineTypes
+// open EngineCore
+// open L0Types
+// open L0Core
+
+module G = FStar.Ghost
+// module PCM = FStar.PCM
+module SZ = FStar.SizeT
+module U8 = FStar.UInt8
+module U16 = FStar.UInt16
+module U32 = FStar.UInt32
+// module PM = Pulse.Lib.PCMMap
+// module FP = Pulse.Lib.PCM.FractionalPreorder
+// module A = Pulse.Lib.Array
+// module PHT = Pulse.Lib.HashTable.Spec
+#lang-pulse
+
+module I = CDDLTest.DPE.InitializeContextInput
+// module DC = CDDLTest.DPE.DeriveContextInput
+// module SI = CDDLTest.DPE.SignInput
+module CK = CDDLTest.DPE.CertifyKeyInput
+open CDDL.Pulse.Types
+open FStar.Seq
+open DPESlice
+module U8 = FStar.UInt8
+module D = CDDLTest.Destructors
+
+let norm_token = emp
+
+ghost
+fn intro_norm ()
+requires emp
+ensures norm_token
+{ fold norm_token; () }
+
+
+ghost
+fn force_norm ()
+requires norm_token
+ensures emp
+{ unfold norm_token; () }
+
+fn initialize_context
+  (#sid:sid_t)
+  (#t:G.erased trace { trace_valid_for_initialize_context t })
+  (#p:perm)
+  (#w:erased _)
+  (input:Slice.slice U8.t)
+requires 
+  pts_to input #p w **
+  sid_pts_to trace_ref sid t
+returns ok:bool
+ensures (
+  if ok 
+  then (
+    exists* (uds:seq U8.t).
+      initialize_context_client_perm sid uds **
+      pts_to input #p w **
+      pure (I.is_uds_bytes uds w)
+  )
+  else (
+    pts_to input #p w **
+    sid_pts_to trace_ref sid t
+  )  
+)
+{ 
+  let uds_opt = I.parse_initialize_context_input_args input;
+  match uds_opt {
+    None -> {
+      unfold (I.parsed_initialize_context_input);
+      false
+    }
+    Some uds_slice -> {
+      unfold (I.parsed_initialize_context_input);
+      if (Slice.len uds_slice <> EngineTypes.uds_len)
+      {
+        Trade.elim_trade _ _;
+        false
+      }
+      else
+      {
+        DPESlice.initialize_context sid t uds_slice;
+        Trade.elim_trade _ _;
+        true
+      }
+    }
+  }
+}
+
+// noextract
+// let trace_valid_for_derive_child (t:trace)  : prop =
+//   match current_state t, r with
+//   | G_Available (Engine_context_repr _)
+//   | G_Available (L0_context_repr _) -> True
+//   | _ -> False
+
+// fn derive_child
+//   (#sid:sid_t)
+//   (#t:G.erased trace { trace_valid_for_derive_child t })
+//   (#p:perm)
+//   (input:slice U8.t)
+// requires
+//   pts_to input #p w **
+//   sid_pts_to trace_ref sid t
+// returns ok:bool
+// ensures
+//   cond ok
+//   (
+//     derive_child_client_perm sid t rrepr b
+//   )
+//   (
+//     pts_to input #p w **
+//     sid_pts_to trace_ref sid t
+//   )
+//         (ensures fun b ->
+//            derive_child_client_perm sid t rrepr b)
